stuck ...

src/Application.thy
@@ -18,6 +18,46 @@ locale example = finite_event_structure carriers for
                             (\<exists>n' n'' v b. n = Some n' \<and> (i, Deliver, Insert (n', v, b) n'') \<sqsubset>\<^sup>i (i, Broadcast, Insert e n))"
   assumes insert_id_unique: "id1 = id2 \<Longrightarrow> (i, Broadcast, Insert (id1, v1, b1) n1) \<in> set (carriers i) \<Longrightarrow> (j, Broadcast, Insert (id2, v2, b2) n2) \<in> set (carriers j) \<Longrightarrow> v1 = v2 \<and> n1 = n2"
   assumes allowed_delete: "(i, Broadcast, Delete x) \<in> set (carriers i) \<Longrightarrow> (\<exists>n' v b. (i, Deliver, Insert (x, v, b) n') \<sqsubset>\<^sup>i (i, Broadcast, Delete x))"
+  assumes insert_or_delete: "(j, f, m) \<in> set (carriers j) \<Longrightarrow> (\<exists>x. m = Delete x) \<or> (\<exists>x y. m = Insert x y)"
+
+lemma (in example) allowed_delete_deliver:
+  assumes "(i, Deliver, Delete x) \<in> set (carriers i)"
+  shows "\<exists>n' v b. (i, Deliver, Insert (x, v, b) n') \<sqsubset>\<^sup>i (i, Deliver, Delete x)"
+using assms apply -
+  apply(drule delivery_has_a_cause)
+  apply clarsimp
+  apply(frule no_message_lost[where j=i])
+  apply(drule allowed_delete)
+  apply clarsimp
+  apply(frule local_order_carrier_closed)
+  apply clarsimp
+  apply(drule delivery_has_a_cause) back
+  apply clarsimp
+  apply(frule no_message_lost[where j=i]) back
+  apply(drule broadcast_causal[rotated, where j=i])
+  apply force
+  apply force
+done
+  
+lemma (in example) allowed_insert_deliver:
+  assumes "(i, Deliver, Insert e n) \<in> set (carriers i)"
+  shows   "n = None \<or> (\<exists>n' n'' v b. n = Some n' \<and> (i, Deliver, Insert (n', v, b) n'') \<sqsubset>\<^sup>i (i, Deliver, Insert e n))"
+using assms
+  apply -
+  apply(frule delivery_has_a_cause)
+  apply(erule exE)
+  apply(cases n; clarsimp)
+  apply(frule allowed_insert)
+  apply clarsimp
+  apply(frule local_order_carrier_closed)
+  apply clarsimp
+  apply(frule delivery_has_a_cause) back
+  apply clarsimp
+  apply(frule no_message_lost[where j=i]) back
+  apply(drule broadcast_causal[rotated, where j=i])
+  apply force
+  apply force
+done
 
 lemma (in example) 
   assumes "fst e1 = fst e2"
@@ -114,15 +154,175 @@ lemma (in example) insert_no_failure:
 using assms
 oops
 
+lemma prefix_set_mem:
+  assumes "xs@ys = zs"
+          "x \<in> set ys"
+  shows   "x \<in> set zs"
+using assms by auto
+
+definition (in example) apply_operations :: "(nat \<times> event_type \<times> (('id \<times> 'v \<times> bool) list \<Rightarrow> ('id \<times> 'v \<times> bool) list)) list \<Rightarrow> ('id \<times> 'v \<times> bool) list" where
+  "apply_operations opers \<equiv> (fold (op \<circ>) (ordered_node_operations opers) id) []"
+
+lemma (in finite_event_structure) carriers_head_lt:
+  assumes "y#ys = carriers i"
+  shows   "\<not>(x \<sqsubset>\<^sup>i y)"
+using assms
+  apply -
+  apply clarsimp
+  apply(subst (asm) carriers_compatible[symmetric])
+  apply clarsimp
+sorry
+
+lemma (in example) apply_operations_singleton:
+  assumes "es = apply_operations [oper]"
+          "oper#ys = carriers i"
+  shows   "\<exists>j e m. oper = (i, e, Insert j m) \<and> (e = Broadcast \<longrightarrow> es = []) \<and> (e = Deliver \<longrightarrow> es = [j])"
+using assms
+  apply(clarsimp simp add: apply_operations_def ordered_node_operations_def)
+  apply(case_tac oper; clarsimp)
+  apply(subgoal_tac "a=i")
+  apply(case_tac b; clarsimp)
+prefer 3
+  using carriers_message_consistent apply (metis list.set_intros(1))
+  apply(subgoal_tac "(i, Broadcast, c) \<in> set (carriers i)")
+  apply(erule disjE[OF insert_or_delete])
+  apply clarsimp
+  apply(subgoal_tac "(i, Broadcast, Delete x) \<in> set (carriers i)")
+  apply(drule allowed_delete)
+  apply clarsimp
+  using carriers_head_lt apply force
+  apply (metis list.set_intros(1))
+  apply force
+  apply (metis list.set_intros(1))
+  apply(subgoal_tac "(i, Deliver, c) \<in> set (carriers i)")
+  apply(erule disjE[OF insert_or_delete])
+  apply clarsimp
+  apply(subgoal_tac "(i, Deliver, Delete x) \<in> set (carriers i)")
+  apply(frule delivery_has_a_cause, erule exE)
+  apply(drule broadcast_before_delivery[where j=i])
+  apply(drule allowed_delete_deliver, clarsimp)
+  using carriers_head_lt apply force
+  apply (metis list.set_intros(1))
+  apply clarsimp
+  apply(rule_tac x=a in exI, rule_tac x=aa in exI, rule_tac x=b in exI)
+  apply(rule conjI)
+  apply force
+  apply(subgoal_tac "y=None", clarsimp)
+  apply(clarsimp simp add: Insert_def)
+  apply(subgoal_tac "(i, Deliver, Insert (a, aa, b) y) \<in> set (carriers i)")
+  apply(drule allowed_insert_deliver)
+  apply(erule disjE, assumption)
+  apply clarsimp
+  using carriers_head_lt apply force  
+  apply (metis list.set_intros(1))+
+done
+
+lemma (in example) apply_operations_singleton_Broadcast:
+  shows "apply_operations (xs @ [(i, Broadcast, f)]) = apply_operations xs"
+by(clarsimp simp add: apply_operations_def ordered_node_operations_def)
+
+lemma (in example) apply_operations_singleton_Deliver:
+  shows "apply_operations (xs @ [(i, Deliver, f)]) = f (apply_operations xs)"
+  apply(clarsimp simp add: apply_operations_def ordered_node_operations_def)
+done
 
 lemma (in example)
-  assumes "{(i, Deliver, Insert e n), (i, Deliver, Insert e' n')} \<subseteq> set (carriers i)"
-          "hb.concurrent (Insert e n) (Insert e' n')"
-  shows   "Insert e n \<circ> Insert e' n' = Insert e' n' \<circ> Insert e n"
+  assumes "\<exists>v b. (m, v, b) \<in> set (apply_operations xs)"
+  shows "map fst (Delete m (apply_operations xs)) = map fst (apply_operations xs)"
+using assms
+  apply(induction xs rule: rev_induct)
+  apply(clarsimp simp add: Delete_def apply_operations_def ordered_node_operations_def)
+  apply clarsimp
+  apply(case_tac aa; clarsimp)
+  apply(subst apply_operations_singleton_Broadcast)+
+  apply(subst (asm) apply_operations_singleton_Broadcast)
+  apply clarsimp apply force
+  apply(subst apply_operations_singleton_Deliver)+
+  apply(subst (asm) apply_operations_singleton_Deliver)
+  apply(unfold Delete_def)
+sorry
+
+lemma (in example) deliver_delete_neq_head:
+  shows "carriers i \<noteq> (i, Deliver, Delete e)#ys"
+  apply clarsimp
+  apply(subgoal_tac "(i, Deliver, Delete e) \<in> set (carriers i)")
+  apply(drule sym)
+  apply(frule delivery_has_a_cause)
+  apply clarsimp
+  apply(drule allowed_delete)
+  apply clarsimp
+  apply(frule local_order_carrier_closed)
+  apply clarsimp
+  apply(drule delivery_has_a_cause) back
+  apply clarsimp
+  apply(frule no_message_lost[where j=i]) back
+  apply(drule broadcast_causal[rotated, where j=i])
+  apply force
+  using carriers_head_lt apply blast
+  apply force
+done
+
+lemma (in example)
+  assumes "\<exists>ys. xs@(i, Deliver, Delete e)#ys = carriers i"
+  shows   "\<exists>v b. (e, v, b) \<in> set (apply_operations xs)"
+using assms
+  apply -
+  apply clarsimp
+  apply(induction xs rule: rev_induct)
+  apply clarsimp
+  using deliver_delete_neq_head apply metis
+  apply clarsimp
+(*
+  apply(drule apply_operations_singleton[rotated], rule refl)  
+  apply clarsimp
+  using deliver_delete_neq_head
+*)
+
+lemma (in example)
+  assumes "\<exists>xs ys. xs@(i, Deliver, Insert e p)#ys = carriers i"
+          "\<exists>zs. prefix@zs = carriers i"
+  shows   "e \<notin> set (apply_operations prefix)"
+using assms 
+  apply -
+  apply clarsimp
+  apply(induction prefix rule: rev_induct)
+  apply(clarsimp simp add: apply_operations_def ordered_node_operations_def)
+  apply clarsimp
+  apply(erule_tac x=xsa in meta_allE, erule_tac x="(a,aa,b)#zs" in meta_allE, erule_tac x="ys" in meta_allE)
+  apply clarsimp
+  apply(case_tac aa; clarsimp)
+  apply(clarsimp simp add: apply_operations_singleton_Broadcast)
+  apply(clarsimp simp add: apply_operations_singleton_Deliver)
+  apply(erule disjE[OF insert_or_delete])
+
+lemma (in example) distinct_ordered_node_operations_prefix:
+  assumes "\<exists>ys. prefix@ys = carriers i"
+  shows   "distinct (map fst (apply_operations prefix))"
+using assms
+  apply -
+  apply(induction prefix rule: rev_induct)
+  apply(clarsimp simp add: ordered_node_operations_def apply_operations_def)+
+  apply(case_tac aa; clarsimp)
+  apply(subgoal_tac "\<exists>ys. xs @ ys = carriers i", clarsimp)
+  apply force
+  apply(subgoal_tac "\<exists>ys. xs @ ys = carriers i", clarsimp)
+
+lemma (in example)
+  assumes "es = apply_operations prefix"
+          "\<exists>ys. prefix@ys = carriers i"
+  
+
+
+  shows   "\<exists>j e m. oper = (i, e, Insert j m) \<and> (e = Broadcast \<longrightarrow> es = []) \<and> (e = Deliver \<longrightarrow> es = [j])"
+
+
+lemma (in example)
+  assumes "hb.concurrent (Insert e n) (Insert e' n')"
+          "\<exists>ys. prefix@ys = carriers i \<and> {(i, Deliver, Insert e n), (i, Deliver, Insert e' n')} \<subseteq> set ys"
+          "xs = apply_operations prefix"
+  shows   "(Insert e n \<circ> Insert e' n') xs = (Insert e' n' \<circ> Insert e n) xs"
 using assms
 apply (subst Insert_def)+
-apply (rule ext)
-apply (rename_tac xs)
 apply clarsimp
 apply (insert insert_commutes[of e e' _ n n'])
 apply (erule_tac x=xs in meta_allE)
@@ -138,18 +338,27 @@ apply clarsimp
 defer
 defer
 
+apply(subgoal_tac "(i, Deliver, Insert e' n') \<in> set (carriers i)")
+apply(subgoal_tac "(i, Deliver, Insert e n) \<in> set (carriers i)")
 apply (rule insert_commute_assms)
 apply clarsimp
 apply (rule conjI)
 apply assumption+
 apply clarsimp
+apply(rule prefix_set_mem, assumption, assumption)+
 
+apply(subgoal_tac "(i, Deliver, Insert e' n') \<in> set (carriers i)")
+apply(subgoal_tac "(i, Deliver, Insert e n) \<in> set (carriers i)")
 apply (rule insert_commute_assms)
 apply clarsimp
 apply (rule conjI)
 apply assumption+
 apply clarsimp
+apply(rule prefix_set_mem, assumption, assumption)+
+
+apply(rule distinct_ordered_node_operations_prefix[where i="i"])
 defer
+
 
 sorry
 
